allocator/slabs bottom-up 16/n
making progress on slot allocation
using Aymeric branch + small trick
verification ok on F*@47a8fe7

src/SlabsUtils.fst
@@ -20,6 +20,7 @@ module SM = Steel.Memory
 
 open Utils2
 open SteelUtils
+//open SteelFix
 
 //TODO: FIXME
 #push-options "--z3rlimit 50"
@@ -209,6 +210,100 @@ let slab_vprop_aux
     (slab_vprop_aux_f_lemma size_class md_as_seq arr)
     incr_seq
 
+let slab_vprop_aux_unpack
+  (size_class: sc)
+  (arr: array U8.t{A.length arr = U32.v page_size})
+  (md_as_seq: G.erased (Seq.lseq U64.t 4))
+  : Steel unit
+  (slab_vprop_aux size_class arr (G.reveal md_as_seq))
+  (fun _ ->
+    starseq
+      #(pos:U32.t{U32.v pos < U32.v (nb_slots size_class)})
+      #(option (Seq.seq U8.t))
+      (slab_vprop_aux_f size_class md_as_seq arr)
+      (slab_vprop_aux_f_lemma size_class md_as_seq arr)
+      (SeqUtils.init_u32_refined (U32.v (nb_slots size_class)))
+  )
+  (requires fun _ -> True)
+  (ensures fun h0 _ h1 ->
+    h0 (slab_vprop_aux size_class arr (G.reveal md_as_seq))
+    ==
+    h1 (starseq
+      #(pos:U32.t{U32.v pos < U32.v (nb_slots size_class)})
+      #(option (Seq.seq U8.t))
+      (slab_vprop_aux_f size_class md_as_seq arr)
+      (slab_vprop_aux_f_lemma size_class md_as_seq arr)
+      (SeqUtils.init_u32_refined (U32.v (nb_slots size_class)))
+    )
+  )
+  =
+  change_slprop_rel
+    (slab_vprop_aux size_class arr md_as_seq)
+    (starseq
+      #(pos:U32.t{U32.v pos < U32.v (nb_slots size_class)})
+      #(option (Seq.seq U8.t))
+      (slab_vprop_aux_f size_class md_as_seq arr)
+      (slab_vprop_aux_f_lemma size_class md_as_seq arr)
+      (SeqUtils.init_u32_refined (U32.v (nb_slots size_class))))
+    (fun x y -> x == y)
+    (fun _ -> ())
+
+let slab_vprop_aux_pack
+  (size_class: sc)
+  (arr: array U8.t{A.length arr = U32.v page_size})
+  (md_as_seq: G.erased (Seq.lseq U64.t 4))
+  : Steel unit
+  (starseq
+    #(pos:U32.t{U32.v pos < U32.v (nb_slots size_class)})
+    #(option (Seq.seq U8.t))
+    (slab_vprop_aux_f size_class md_as_seq arr)
+    (slab_vprop_aux_f_lemma size_class md_as_seq arr)
+    (SeqUtils.init_u32_refined (U32.v (nb_slots size_class))))
+  (fun _ ->
+    slab_vprop_aux size_class arr (G.reveal md_as_seq)
+  )
+  (requires fun _ -> True)
+  (ensures fun h0 _ h1 ->
+    h1 (slab_vprop_aux size_class arr (G.reveal md_as_seq))
+    ==
+    h0 (starseq
+      #(pos:U32.t{U32.v pos < U32.v (nb_slots size_class)})
+      #(option (Seq.seq U8.t))
+      (slab_vprop_aux_f size_class md_as_seq arr)
+      (slab_vprop_aux_f_lemma size_class md_as_seq arr)
+      (SeqUtils.init_u32_refined (U32.v (nb_slots size_class)))
+    )
+  )
+  =
+  change_slprop_rel
+    (starseq
+      #(pos:U32.t{U32.v pos < U32.v (nb_slots size_class)})
+      #(option (Seq.seq U8.t))
+      (slab_vprop_aux_f size_class md_as_seq arr)
+      (slab_vprop_aux_f_lemma size_class md_as_seq arr)
+      (SeqUtils.init_u32_refined (U32.v (nb_slots size_class))))
+    (slab_vprop_aux size_class arr md_as_seq)
+    (fun x y -> x == y)
+    (fun _ -> ())
+
+let slab_vprop_aux_idem
+  (size_class: sc)
+  (arr: array U8.t{A.length arr = U32.v page_size})
+  (md_as_seq: G.erased (Seq.lseq U64.t 4))
+  : Steel unit
+  (slab_vprop_aux size_class arr (G.reveal md_as_seq))
+  (fun _ -> slab_vprop_aux size_class arr (G.reveal md_as_seq))
+  (requires fun _ -> True)
+  (ensures fun h0 _ h1 ->
+    h1 (slab_vprop_aux size_class arr (G.reveal md_as_seq))
+    ==
+    h0 (slab_vprop_aux size_class arr (G.reveal md_as_seq))
+  )
+  =
+  slab_vprop_aux_unpack size_class arr md_as_seq;
+  slab_vprop_aux_pack size_class arr md_as_seq;
+  return ()
+
 //unfold
 //[@@__steel_reduce__]
 let slab_vprop
@@ -218,12 +313,14 @@ let slab_vprop
   =
   A.varray md `vdep` (fun (md_as_seq: Seq.lseq U64.t 4) -> slab_vprop_aux size_class arr md_as_seq)
 
+
 //works
 let slab_vprop1
   (md: slab_metadata)
   =
   reveal_emp ();
-  emp `vdep` (fun (_:unit) -> emp)
+  assume (normal (t_of emp) == unit);
+  emp `vdep` (fun _ -> emp)
 
 //works
 let slab_vprop2
@@ -240,7 +337,7 @@ let slab_vprop4_aux
   = fun (x: Seq.lseq U64.t 4) -> emp
 
 let slab_vprop4
-  (md: slab_metadata)
+  (md: array U64.t{A.length md = 4})
   =
   A.varray md `vdep`
     (fun (x: Seq.lseq U64.t 4) -> slab_vprop4_aux x)
@@ -251,10 +348,77 @@ let slab_vprop_test
 
 #push-options "--print_implicits"
 
+let t (md: array U64.t)
+  : Lemma
+  (requires A.length md = 4)
+  (ensures
+    //normal (t_of (A.varray md)) == Seq.lseq U64.t 4
+    t_of (A.varray md) == Seq.lseq U64.t 4
+  )
+  = ()
+
+inline_for_extraction
+let elim_intro_vdep_test_aux
+  (size_class: sc)
+  (md: array U64.t{A.length md = 4})
+  (md_as_seq: G.erased (Seq.lseq U64.t 4))
+  (arr: array U8.t{A.length arr = U32.v page_size})
+  (pos: U32.t{U32.v pos < U32.v (nb_slots size_class)})
+  : Steel unit
+  (
+  A.varray md `star`
+  starseq
+    #(pos:U32.t{U32.v pos < U32.v (nb_slots size_class)})
+    #(option (Seq.seq U8.t))
+    (slab_vprop_aux_f size_class md_as_seq arr)
+    (slab_vprop_aux_f_lemma size_class md_as_seq arr)
+    (SeqUtils.init_u32_refined (U32.v (nb_slots size_class)))
+  )
+  (
+  fun _ -> A.varray md `star`
+  starseq
+    #(pos:U32.t{U32.v pos < U32.v (nb_slots size_class)})
+    #(option (Seq.seq U8.t))
+    (slab_vprop_aux_f size_class md_as_seq arr)
+    (slab_vprop_aux_f_lemma size_class md_as_seq arr)
+    (SeqUtils.init_u32_refined (U32.v (nb_slots size_class)))
+  )
+  (requires fun h0 ->
+    A.asel md h0 == G.reveal md_as_seq
+  )
+  (ensures fun h0 _ h1 ->
+    let v0 = A.asel md h0 in
+    let v1 = A.asel md h1 in
+    let bm0 = Bitmap4.array_to_bv2 v0 in
+    let bm1 = Bitmap4.array_to_bv2 v1 in
+    let idx = Bitmap5.f #4 (U32.v pos) in
+    v0 == v1 /\
+    bm1 == bm0 /\
+    v_starseq
+      #(pos:U32.t{U32.v pos < U32.v (nb_slots size_class)})
+      #(option (Seq.seq U8.t))
+      (slab_vprop_aux_f size_class md_as_seq arr)
+      (slab_vprop_aux_f_lemma size_class md_as_seq arr)
+      (SeqUtils.init_u32_refined (U32.v (nb_slots size_class)))
+      h0
+    ==
+    v_starseq
+      #(pos:U32.t{U32.v pos < U32.v (nb_slots size_class)})
+      #(option (Seq.seq U8.t))
+      (slab_vprop_aux_f size_class md_as_seq arr)
+      (slab_vprop_aux_f_lemma size_class md_as_seq arr)
+      (SeqUtils.init_u32_refined (U32.v (nb_slots size_class)))
+      h1)
+  =
+  admit ();
+  return ()
+
+
 let elim_intro_vdep_test
   (size_class: sc)
   (md: slab_metadata)
   (arr: array U8.t{A.length arr = U32.v page_size})
+  (pos: U32.t{U32.v pos < U32.v (nb_slots size_class)})
   : Steel unit
   (slab_vprop size_class arr md)
   (fun r -> slab_vprop size_class arr md)
@@ -265,11 +429,31 @@ let elim_intro_vdep_test
     h0 (slab_vprop size_class arr md)
   )
   =
+  assert (t_of (A.varray md) == Seq.lseq U64.t 4);
+  //let md_as_seq : G.erased (normal (t_of (A.varray md))) = elim_vdep
+  //let md_as_seq : G.erased (Seq.lseq U64.t 4) = elim_vdep
   let md_as_seq = elim_vdep
     (A.varray md)
-    (fun (x:Seq.lseq U64.t 4) -> slab_vprop_aux size_class arr x) in
+    (fun (x: Seq.lseq U64.t 4) -> slab_vprop_aux size_class arr x)
+  in
+  let md_as_seq2 = G.hide ((G.reveal md_as_seq) <: Seq.lseq U64.t 4) in
+  change_slprop_rel
+    (slab_vprop_aux size_class arr md_as_seq)
+    (slab_vprop_aux size_class arr md_as_seq2)
+    (fun x y -> x == y)
+    (fun _ -> ());
+  slassert (A.varray md `star` slab_vprop_aux size_class arr (G.reveal md_as_seq2));
+  //slab_vprop_aux_idem size_class arr md_as_seq2;
+  slab_vprop_aux_unpack size_class arr md_as_seq2;
+  elim_intro_vdep_test_aux
+    size_class
+    md
+    md_as_seq2
+    arr
+    pos;
+  slab_vprop_aux_pack size_class arr md_as_seq2;
   intro_vdep
     (A.varray md)
-    (slab_vprop_aux size_class arr md_as_seq)
-    (fun (x:Seq.lseq U64.t 4) -> slab_vprop_aux size_class arr x);
+    (slab_vprop_aux size_class arr md_as_seq2)
+    (fun (x: Seq.lseq U64.t 4) -> slab_vprop_aux size_class arr x);
   return ()
